src/coq/Theory/ExpLemmas.v
@@ -34,6 +34,13 @@ From Vellvm Require Import
 Import D.
 Open Scope itree_scope.
 
+Notation "'ℑ'" := interp_cfg_to_L3. 
+Notation "'Θ'" := (translate exp_E_to_instr_E).
+Notation "⟦ e : t ⟧" := (denote_exp t e).
+Notation "⟦ e : t ⟧" := (denote_exp (Some t) e).
+Notation "⟦ e ⟧" := (denote_exp None e).
+Import ITreeNotations.
+
 Section Translations.
 
   (* Technicality: translations by [lookup_E_to_exp_E] and [exp_E_to_instr_E] leave these events unphased *)
@@ -66,7 +73,37 @@ Section Translations.
   Proof.
     reflexivity.
   Qed.
-  
+
+  Lemma exp_E_to_instr_E_Pick : forall {X} (e : PickE X),
+      exp_E_to_instr_E (subevent X e) = subevent X e.
+  Proof.
+    reflexivity.
+  Qed.
+
+  Lemma exp_E_to_instr_E_UB : forall {X} (e : UBE X),
+      exp_E_to_instr_E (subevent X e) = subevent X e.
+  Proof.
+    reflexivity.
+  Qed.
+
+  Lemma exp_E_to_instr_E_Fail : forall {X} (e : FailureE X),
+      exp_E_to_instr_E (subevent X e) = subevent X e.
+  Proof.
+    reflexivity.
+  Qed.
+
+  Lemma _failure_UB_to_ExpE_UB : forall {X} (e : UBE X),
+      _failure_UB_to_ExpE (subevent X e) = subevent X e.
+  Proof.
+    reflexivity.
+  Qed.
+
+  Lemma _failure_UB_to_ExpE_fail : forall {X} (e : FailureE X),
+      _failure_UB_to_ExpE (subevent X e) = subevent X e.
+  Proof.
+    reflexivity.
+  Qed.
+
 End Translations.
 
 Lemma denote_exp_GR :forall g l m id v τ,
@@ -443,11 +480,26 @@ Proof.
   reflexivity.
 Qed.
 
+(* TODO MOVE *)
+Definition state_cfg : Type := memory_stack * (local_env * global_env).
+
+Definition state_cfg_T (T:Type): Type
+  := memory_stack * (local_env * (global_env * T)).
+
+Definition state_cfgP := state_cfg -> Prop.
+Definition state_cfg_TP {T : Type} := state_cfg_T T -> Prop.
+Definition lift_state_cfgP {T : Type} (P : state_cfgP) : @state_cfg_TP T :=
+  fun '(m,(l,(g,_))) => P (m,(l,g)).
+
+Notation "↑" :=  lift_state_cfgP.
+
 (* Expressions are "almost pure" computations:
    they depend on the memory, but do not modify any component on the state *)
 
+Definition pure_P g l m : state_cfgP := fun '(m',(l',g')) => m' = m /\ l' = l /\ g' = g.
+
 Definition pure {E R} (t : global_env -> local_env -> memory_stack -> itree E (memory_stack * (local_env * (global_env * R)))) : Prop :=
-  forall g l m, t g l m ⤳ fun '(m',(l',(g',_))) => m' = m /\ l' = l /\ g' = g.
+  forall g l m, t g l m ⤳ ↑ (pure_P g l m).
 
 Require Import String.
 Opaque append.
@@ -455,36 +507,115 @@ Opaque append.
 Lemma failure_is_pure : forall R s,
     pure (R := R) (interp_cfg_to_L3 (translate exp_E_to_instr_E (raise s))).
 Proof.
-  unfold pure, has_post, raise, Exception.throw; intros.
-  rewrite translate_vis.
+  unfold pure, raise; intros.
+  rewrite translate_bind,translate_trigger, exp_E_to_instr_E_Fail, subevent_subevent, interp_cfg_to_L3_bind.
   unfold interp_cfg_to_L3.
-  rewrite interp_intrinsics_vis.
-  cbn; unfold Intrinsics.F_trigger; cbn; rewrite subevent_subevent.
-  rewrite interp_global_bind, interp_global_trigger.
-  cbn; rewrite subevent_subevent.
-  rewrite !interp_local_bind, interp_local_trigger.
-  cbn; rewrite subevent_subevent.
-  rewrite !interp_memory_bind, interp_memory_trigger.
+  rewrite interp_intrinsics_trigger.
   cbn.
-  apply eutt_eq_bind; intros (_ & ? & ? & []).
+  unfold Intrinsics.F_trigger; cbn.
+  rewrite subevent_subevent.
+  rewrite interp_global_trigger; cbn.
+  rewrite subevent_subevent.
+  rewrite interp_local_bind, interp_local_trigger; cbn.
+  rewrite subevent_subevent, bind_bind.
+  rewrite interp_memory_bind, interp_memory_trigger; cbn.
+  rewrite subevent_subevent, !bind_bind.
+  apply has_post_bind; intros [].
+Qed.
+
+Lemma interp_cfg_to_L3_pick : forall u P m l g,
+    interp_cfg_to_L3 (trigger (pick u P)) g l m ≈ v <- trigger (pick u P);; Ret (m,(l,(g,v))).
+Proof.
+  intros.
+  unfold interp_cfg_to_L3.
+  rewrite interp_intrinsics_trigger.
+  cbn.
+  unfold Intrinsics.F_trigger; cbn.
+  rewrite subevent_subevent.
+  rewrite interp_global_trigger; cbn.
+  rewrite subevent_subevent.
+  rewrite interp_local_bind, interp_local_trigger; cbn.
+  rewrite subevent_subevent, bind_bind.
+  rewrite interp_memory_bind, interp_memory_trigger; cbn.
+  rewrite subevent_subevent, bind_bind.
+  apply eutt_eq_bind; intros.
+  rewrite bind_ret_l.
+  rewrite interp_memory_bind, interp_memory_ret, bind_ret_l; cbn.
+  rewrite interp_local_ret, interp_memory_ret.
+  reflexivity.
+Qed.
+
+Lemma interp_cfg_to_L3_UB : forall s m l g,
+    interp_cfg_to_L3 (trigger (ThrowUB s)) g l m ≈ v <- trigger (ThrowUB s);; Ret (m,(l,(g,v))).
+Proof.
+  intros.
+  unfold interp_cfg_to_L3.
+  rewrite interp_intrinsics_trigger.
+  cbn.
+  unfold Intrinsics.F_trigger; cbn.
+  rewrite subevent_subevent.
+  rewrite interp_global_trigger; cbn.
+  rewrite subevent_subevent.
+  rewrite interp_local_bind, interp_local_trigger; cbn.
+  rewrite subevent_subevent, bind_bind.
+  rewrite interp_memory_bind, interp_memory_trigger; cbn.
+  rewrite subevent_subevent, bind_bind.
+  apply eutt_eq_bind; intros.
+  rewrite bind_ret_l.
+  rewrite interp_memory_bind, interp_memory_ret, bind_ret_l; cbn.
+  rewrite interp_local_ret, interp_memory_ret.
+  reflexivity.
+Qed.
+
+Lemma pick_is_pure : forall u P, pure (ℑ (Θ (trigger (pick u P)))).
+Proof.
+  intros.
+  unfold pure; intros. 
+  rewrite translate_trigger.
+  rewrite exp_E_to_instr_E_Pick, subevent_subevent.
+  rewrite interp_cfg_to_L3_pick.
+  apply has_post_bind.
+  intros ?; apply eutt_Ret; cbn; auto.
+Qed.
+
+Lemma concretize_or_pick_is_pure : forall v P, pure (ℑ (Θ (concretize_or_pick v P))).
+Proof.
+  intros.
+  unfold pure; intros.
+  unfold concretize_or_pick.
+  break_match_goal; [| apply pick_is_pure].
+  unfold lift_err.
+  break_match_goal; [apply failure_is_pure |].
+  cbn.
+  rewrite !translate_ret, interp_cfg_to_L3_ret.
+  apply eutt_Ret; cbn; auto.
 Qed.
 
 Lemma UB_is_pure : forall R s,
     pure (R := R) (interp_cfg_to_L3 (translate exp_E_to_instr_E (raiseUB s))).
 Proof.
-  unfold pure, has_post, raiseUB; intros.
-  rewrite translate_vis.
-  unfold interp_cfg_to_L3.
-  rewrite interp_intrinsics_vis.
-  cbn; unfold Intrinsics.F_trigger; cbn; rewrite subevent_subevent.
-  rewrite interp_global_bind, interp_global_trigger.
-  cbn; rewrite subevent_subevent.
-  rewrite !interp_local_bind, interp_local_trigger.
-  cbn; rewrite subevent_subevent.
-  rewrite !interp_memory_bind, interp_memory_trigger.
-  cbn.
-  apply eutt_eq_bind; intros (_ & ? & ? & []).
+  unfold pure, raiseUB; intros.
+  rewrite translate_bind, translate_trigger, exp_E_to_instr_E_UB, subevent_subevent.
+  rewrite interp_cfg_to_L3_bind, interp_cfg_to_L3_UB.
+  apply has_post_bind.
+  intros (? & ? & ? & []).
 Qed.
+
+Lemma translate_raiseUB : forall T s,
+    translate _failure_UB_to_ExpE (raiseUB (X := T) s) ≈ raiseUB s.
+Proof.
+  intros.
+  unfold raiseUB; rewrite translate_bind, translate_trigger, _failure_UB_to_ExpE_UB, subevent_subevent.
+  apply eutt_eq_bind; intros [].
+Qed.
+
+Lemma translate_raise : forall T s,
+    translate _failure_UB_to_ExpE (raise (A := T) s) ≈ raise s. Proof.
+  intros.
+  unfold raise; rewrite translate_bind, translate_trigger, _failure_UB_to_ExpE_fail, subevent_subevent.
+  apply eutt_eq_bind; intros [].
+Qed.
+
 
 Lemma translate_map_monad {E F A B} (l : list A) (ts : A -> itree E B) (h : E ~> F) :
   translate h (map_monad ts l) ≈ map_monad (fun a => translate h (ts a)) l.
@@ -538,80 +669,122 @@ Qed.
 
 Lemma map_monad_eutt_state_ind :
   forall {E S A B} (I : S -> Prop) (f : A -> Monads.stateT S (itree E) B) (l : list A) s,
-    (forall a s, In a l -> (f a s) ⤳ fun '(s,_) => I s) ->
+    (forall a s, In a l -> I s -> (f a s) ⤳ fun '(s,_) => I s) ->
     I s ->
     map_monad f l s ⤳ fun '(s,_) => I s.
 Proof.
   induction l as [| a l IH]; intros s HB HI; simpl.
   - apply eutt_Ret; auto.
   - setoid_rewrite has_post_post_strong in HB.
-    eapply eutt_clo_bind; [apply HB; left; auto |].
+    eapply eutt_clo_bind; [apply HB; cbn; auto |].
     intros [s' ?] [] [EQ ?]; inv EQ.
     simpl.
     setoid_rewrite has_post_post_strong in IH.
     eapply eutt_clo_bind; [apply IH |]; auto.
-    intros; apply HB; right; auto.
+    intros; apply HB; cbn; auto. 
     intros [s' ?] [] [EQ ?]; inv EQ; cbn; apply eutt_Ret; auto. 
 Qed.
 
-(* Lemma map_monad_L3_ind : *)
-(*   forall {A B} (I : S -> Prop) (f : A -> Monads.stateT S (itree E) B) (l : list A) s, *)
-(*     (forall a s, In a l -> (f a s) ⤳ fun '(s,_) => I s) -> *)
-(*     I s -> *)
-(*     map_monad f xs g l m ⤳ fun '(s,_) => I s. *)
-(* Proof. *)
-(*   induction l as [| a l IH]; intros s HB HI; simpl. *)
-(*   - apply eutt_Ret; auto. *)
-(*   - setoid_rewrite has_post_post_strong in HB. *)
-(*     eapply eutt_clo_bind; [apply HB; left; auto |]. *)
-(*     intros [s' ?] [] [EQ ?]; inv EQ. *)
-(*     simpl. *)
-(*     setoid_rewrite has_post_post_strong in IH. *)
-(*     eapply eutt_clo_bind; [apply IH |]; auto. *)
-(*     intros; apply HB; right; auto. *)
-(*     intros [s' ?] [] [EQ ?]; inv EQ; cbn; apply eutt_Ret; auto.  *)
-(* Qed. *)
+Lemma map_monad_eutt_state2_ind :
+  forall {E S1 S2 A B} (I : S1 -> S2 -> Prop)
+    (f : A -> Monads.stateT S1 (Monads.stateT S2 (itree E)) B)
+    (l : list A) (s1 : S1) (s2 : S2), 
+    (forall a s1 s2, In a l -> I s1 s2 -> (f a s1 s2) ⤳ fun '(s2',(s1',_)) => I s1' s2') ->
+    I s1 s2 ->
+    map_monad f l s1 s2 ⤳ fun '(s2',(s1',_)) => I s1' s2'.
+Proof.
+  induction l as [| a l IH]; intros s1 s2 HB HI; simpl.
+  - apply eutt_Ret; auto.
+  - setoid_rewrite has_post_post_strong in HB.
+    eapply eutt_clo_bind; [apply HB; cbn; auto |].
+    intros (s2' & s1' & ?) (? & ? & ?) [EQ ?]; inv EQ.
+    simpl.
+    setoid_rewrite has_post_post_strong in IH.
+    eapply eutt_clo_bind; [apply IH |]; auto.
+    intros; apply HB; cbn; auto.
+    intros (s1' & s2' & ?) (? & ? & ?) [EQ ?]; inv EQ; cbn; apply eutt_Ret; auto. 
+Qed.
+
+Lemma map_monad_eutt_state3_ind :
+  forall {E S1 S2 S3 A B} (I : S1 -> S2 -> S3 -> Prop)
+    (f : A -> Monads.stateT S1 (Monads.stateT S2 (Monads.stateT S3 (itree E))) B)
+    (l : list A) (s1 : S1) (s2 : S2) (s3 : S3), 
+    (forall a s1 s2 s3, In a l -> I s1 s2 s3 -> (f a s1 s2 s3) ⤳ fun '(s3', (s2',(s1',_))) => I s1' s2' s3') ->
+    I s1 s2 s3 ->
+    map_monad f l s1 s2 s3 ⤳ fun '(s3', (s2',(s1',_))) => I s1' s2' s3'.
+Proof.
+  induction l as [| a l IH]; intros s1 s2 s3 HB HI; simpl.
+  - apply eutt_Ret; auto.
+  - setoid_rewrite has_post_post_strong in HB.
+    eapply eutt_clo_bind; [apply HB; cbn; auto |].
+    intros (s3' & s2' & s1' & ?) (? & ? & ? & ?) [EQ ?]; inv EQ.
+    simpl.
+    setoid_rewrite has_post_post_strong in IH.
+    eapply eutt_clo_bind; [apply IH |]; auto.
+    intros; apply HB; cbn; auto.
+    intros (s1' & s2' & s3' & ?) (? & ? & ? & ?) [EQ ?]; inv EQ; cbn; apply eutt_Ret; auto. 
+Qed.
+
+Lemma interp_cfg_to_L3_GR_fail : forall id g l m,
+    Maps.lookup id g = None ->
+    interp_cfg_to_L3 (trigger (GlobalRead id)) g l m ≈
+                     raise ("Could not look up global id " ++ CeresSerialize.to_string id).
+Proof.
+  intros * LU.
+  unfold interp_cfg_to_L3.
+  rewrite interp_intrinsics_trigger.
+  cbn.
+  unfold Intrinsics.F_trigger; cbn; rewrite subevent_subevent.
+  rewrite interp_global_trigger. 
+  cbn in *; rewrite LU.
+  unfold raise; cbn.
+  rewrite interp_local_bind, interp_local_trigger; cbn; rewrite subevent_subevent, bind_bind.
+  rewrite interp_memory_bind, interp_memory_trigger; cbn; rewrite subevent_subevent, bind_bind.
+  apply eutt_eq_bind; intros [].
+Qed.
+
+Lemma interp_cfg_to_L3_LR_fail : forall id g l m,
+    Maps.lookup id l = None ->
+    interp_cfg_to_L3 (trigger (LocalRead id)) g l m ≈
+                     raise ("Could not look up id " ++ CeresSerialize.to_string id).
+Proof.
+  intros * LU.
+  unfold interp_cfg_to_L3.
+  rewrite interp_intrinsics_trigger.
+  cbn.
+  unfold Intrinsics.F_trigger; cbn; rewrite subevent_subevent.
+  rewrite interp_global_trigger. 
+  cbn in *; rewrite subevent_subevent.
+  rewrite interp_local_bind, interp_local_trigger.
+  cbn; rewrite LU.
+  unfold raise; cbn; rewrite bind_bind.
+  rewrite interp_memory_bind, interp_memory_trigger; cbn; rewrite subevent_subevent, bind_bind.
+  apply eutt_eq_bind; intros [].
+Qed.
 
 Lemma expr_are_pure : forall o e, pure (interp_cfg_to_L3 (translate exp_E_to_instr_E (denote_exp o e))).
 Proof.
-  intros; unfold pure, has_post.
-  induction e; simpl; intros.
+  intros; unfold pure.
+  revert o; induction e; simpl; intros.
 
   - destruct id; cbn.
     + rewrite translate_bind, translate_trigger, lookup_E_to_exp_E_Global, subevent_subevent.
       rewrite translate_bind, translate_trigger, exp_E_to_instr_E_Global, subevent_subevent.
-      rewrite interp_cfg_to_L3_bind. 
-      unfold interp_cfg_to_L3.
-      rewrite interp_intrinsics_trigger.
-      cbn; unfold Intrinsics.F_trigger; cbn.
-      rewrite interp_global_trigger.
-      cbn.
-      break_match_goal; cbn.
-      * rewrite interp_local_ret, interp_memory_ret, bind_ret_l.
-        rewrite !translate_ret, interp_intrinsics_ret, interp_global_ret, interp_local_ret, interp_memory_ret.
-        apply eutt_Ret; intuition.
-      * unfold raise, Exception.throw.
-        rewrite interp_local_vis.
-        cbn; rewrite !bind_bind.
-        rewrite interp_memory_bind, interp_memory_trigger.
-        cbn.
-        rewrite !bind_bind.
-        apply eutt_eq_bind; intros [].
+      destruct (Maps.lookup id g) eqn:EQ.
+      * rewrite interp_cfg_to_L3_bind, interp_cfg_to_L3_GR; eauto.
+        rewrite bind_ret_l, !translate_ret, interp_cfg_to_L3_ret.
+        apply eutt_Ret; cbn; auto.
+      * rewrite interp_cfg_to_L3_bind, interp_cfg_to_L3_GR_fail; auto.
+        unfold raise; rewrite bind_bind.
+        apply has_post_bind; intros [].
+        
     + rewrite translate_trigger, lookup_E_to_exp_E_Local, subevent_subevent.
-      rewrite translate_trigger, exp_E_to_instr_E_Local, subevent_subevent.
-      unfold interp_cfg_to_L3.
-      rewrite interp_intrinsics_trigger.
-      cbn; unfold Intrinsics.F_trigger; cbn.
-      rewrite interp_global_trigger.
-      cbn.
-      rewrite interp_local_bind, interp_local_trigger.
-      cbn.
-      break_match_goal; cbn.
-      * rewrite bind_ret_l,interp_local_ret, interp_memory_ret.
-        apply eutt_Ret; intuition.
-      * unfold raise, Exception.throw.
-        rewrite interp_memory_bind, interp_memory_vis, !bind_bind.
-        apply eutt_eq_bind; intros [? []].
+      destruct (Maps.lookup id l) eqn:EQ.
+      * rewrite translate_trigger, exp_E_to_instr_E_Local, subevent_subevent, interp_cfg_to_L3_LR; eauto.
+        apply eutt_Ret; cbn; auto.
+      * rewrite translate_trigger, exp_E_to_instr_E_Local, subevent_subevent, interp_cfg_to_L3_LR_fail; auto. 
+        unfold raise.
+        apply has_post_bind; intros [].
 
   - destruct o; cbn; [| apply failure_is_pure].
     destruct d; simpl.
@@ -620,27 +793,27 @@ Proof.
     cbn.
     break_match_goal; [apply UB_is_pure |].
     break_match_goal; [apply failure_is_pure|]. 
-    rewrite translate_ret, interp_cfg_to_L3_ret; apply eutt_Ret; intuition.
+    rewrite translate_ret, interp_cfg_to_L3_ret; apply eutt_Ret; cbn; intuition.
 
   - destruct o; cbn; [| apply failure_is_pure].
     destruct d; simpl.
     all: match goal with |- context[raise _] => apply failure_is_pure | _ => idtac end.
-    rewrite translate_ret, interp_cfg_to_L3_ret; apply eutt_Ret; intuition.
+    rewrite translate_ret, interp_cfg_to_L3_ret; apply eutt_Ret; cbn; intuition.
 
   - destruct o; cbn; [| apply failure_is_pure].
     destruct d; simpl.
     all: match goal with |- context[raise _] => apply failure_is_pure | _ => idtac end.
-    rewrite translate_ret, interp_cfg_to_L3_ret; apply eutt_Ret; intuition.
+    rewrite translate_ret, interp_cfg_to_L3_ret; apply eutt_Ret; cbn; intuition.
 
   - destruct o; cbn; [| apply failure_is_pure].
     destruct d; simpl.
     all: match goal with |- context[raise _] => apply failure_is_pure | _ => idtac end.
-    rewrite translate_ret, interp_cfg_to_L3_ret; apply eutt_Ret; intuition.
-    rewrite translate_ret, interp_cfg_to_L3_ret; apply eutt_Ret; intuition.
+    rewrite translate_ret, interp_cfg_to_L3_ret; apply eutt_Ret; cbn; intuition.
+    rewrite translate_ret, interp_cfg_to_L3_ret; apply eutt_Ret; cbn; intuition.
 
-  - destruct b; simpl; rewrite translate_ret, interp_cfg_to_L3_ret; apply eutt_Ret; intuition.
+  - destruct b; simpl; rewrite translate_ret, interp_cfg_to_L3_ret; apply eutt_Ret; cbn; intuition.
 
-  - simpl; rewrite translate_ret, interp_cfg_to_L3_ret; apply eutt_Ret; intuition.
+  - simpl; rewrite translate_ret, interp_cfg_to_L3_ret; apply eutt_Ret; cbn; intuition.
 
   - destruct o; cbn; [| apply failure_is_pure].
     apply failure_is_pure.
@@ -648,13 +821,395 @@ Proof.
   - apply failure_is_pure.
 
   - destruct o; cbn; [| apply failure_is_pure].
-    rewrite translate_ret, interp_cfg_to_L3_ret; apply eutt_Ret; intuition.
+    rewrite translate_ret, interp_cfg_to_L3_ret; apply eutt_Ret; cbn; intuition.
 
   - rewrite translate_bind, interp_cfg_to_L3_bind.
     rewrite translate_map_monad.
     rewrite interp_cfg_to_L3_map_monad.
-    (* eapply eutt_clo_bind. *)
-    (* Unshelve. *)
+    apply has_post_bind_strong with (S := ↑ (pure_P g l m)).
+    + eapply has_post_weaken.
+      apply (map_monad_eutt_state3_ind (fun g' l' m' => pure_P g l m (m',(l',g')))); [| cbn; intuition].
+      * intros * IN (-> & -> & ->).
+        destruct a; simpl in *.
+        apply has_post_weaken with (↑ (pure_P g l m)).
+        apply (H _ IN).
+        intros (? & ? & ? & ?) (-> & -> & ->); auto.
+      * intros (? & ? & ? & ?) (-> & -> & ->); cbn; auto.
+    + intros (? & ? & ? & ?) (-> & -> & ->).
+      simpl; rewrite translate_ret, interp_cfg_to_L3_ret; apply eutt_Ret; cbn; intuition.
 
+  - destruct o; cbn; [| apply failure_is_pure].
+    destruct d;
+    match goal with
+      |- context[denote_exp (Some (DTYPE_Packed_struct _))] => idtac 
+    | _ => apply failure_is_pure
+    end.
+    simpl.
+    rewrite translate_bind, interp_cfg_to_L3_bind.
+    rewrite translate_map_monad.
+    rewrite interp_cfg_to_L3_map_monad.
+    apply has_post_bind_strong with (S := ↑ (pure_P g l m)).
+    + eapply has_post_weaken.
+      apply (map_monad_eutt_state3_ind (fun g' l' m' => pure_P g l m (m',(l',g')))); [| cbn; intuition].
+      * intros * IN (-> & -> & ->).
+        destruct a; simpl in *.
+        apply has_post_weaken with (↑ (pure_P g l m)).
+        apply (H _ IN).
+        intros (? & ? & ? & ?) (-> & -> & ->); auto.
+      * intros (? & ? & ? & ?) (-> & -> & ->); cbn; auto.
+    + intros (? & ? & ? & ?) (-> & -> & ->).
+      simpl; rewrite translate_ret, interp_cfg_to_L3_ret; apply eutt_Ret; cbn; intuition.
+
+
+  - rewrite translate_bind, interp_cfg_to_L3_bind.
+    rewrite translate_map_monad.
+    rewrite interp_cfg_to_L3_map_monad.
+    apply has_post_bind_strong with (S := ↑ (pure_P g l m)).
+    + eapply has_post_weaken.
+      apply (map_monad_eutt_state3_ind (fun g' l' m' => pure_P g l m (m',(l',g')))); [| cbn; intuition].
+      * intros * IN (-> & -> & ->).
+        destruct a; simpl in *.
+        apply has_post_weaken with (↑ (pure_P g l m)).
+        apply (H _ IN).
+        intros (? & ? & ? & ?) (-> & -> & ->); auto.
+      * intros (? & ? & ? & ?) (-> & -> & ->); cbn; auto.
+    + intros (? & ? & ? & ?) (-> & -> & ->).
+      simpl; rewrite translate_ret, interp_cfg_to_L3_ret; apply eutt_Ret; cbn; intuition.
+
+  - rewrite translate_bind, interp_cfg_to_L3_bind.
+    rewrite translate_map_monad.
+    rewrite interp_cfg_to_L3_map_monad.
+    apply has_post_bind_strong with (S := ↑ (pure_P g l m)).
+    + eapply has_post_weaken.
+      apply (map_monad_eutt_state3_ind (fun g' l' m' => pure_P g l m (m',(l',g')))); [| cbn; intuition].
+      * intros * IN (-> & -> & ->).
+        destruct a; simpl in *.
+        apply has_post_weaken with (↑ (pure_P g l m)).
+        apply (H _ IN).
+        intros (? & ? & ? & ?) (-> & -> & ->); auto.
+      * intros (? & ? & ? & ?) (-> & -> & ->); cbn; auto.
+    + intros (? & ? & ? & ?) (-> & -> & ->).
+      simpl; rewrite translate_ret, interp_cfg_to_L3_ret; apply eutt_Ret; cbn; intuition.
+
+  - rewrite translate_bind, interp_cfg_to_L3_bind.
+    eapply has_post_bind_strong.
+    apply (IHe1 (Some t) g l m).
+    intros (? & ? & ? & ?) (-> & -> & ->).
+    rewrite translate_bind, interp_cfg_to_L3_bind.
+    eapply has_post_bind_strong.
+    apply (IHe2 (Some t) g l m).
+    intros (? & ? & ? & ?) (-> & -> & ->).
+    break_match_goal.
+    + rewrite translate_bind, interp_cfg_to_L3_bind.
+      apply has_post_bind_strong with (↑ (pure_P g l m)).
+      * unfold concretize_or_pick.
+        break_match_goal.
+        cbn.
+        {
+          unfold lift_err.
+          break_match_goal.
+          apply failure_is_pure.
+          rewrite translate_ret, interp_cfg_to_L3_ret.
+          apply eutt_Ret; cbn; auto.
+        }
+       apply pick_is_pure.
+
+      * intros (? & ? & ? & ?) (-> & -> & ->).
+        unfold uvalue_to_dvalue_binop2.
+        cbn; break_match_goal.
+        rewrite translate_ret, interp_cfg_to_L3_ret.
+        apply eutt_Ret; cbn; auto.
+        break_match_hyp; inv_sum.
+        break_match_goal.
+        rewrite translate_raiseUB; apply UB_is_pure.
+        break_match_goal.
+        rewrite translate_raise; apply failure_is_pure.
+        rewrite !translate_ret, interp_cfg_to_L3_ret.
+        apply eutt_Ret; cbn; auto.
+
+    + unfold uvalue_to_dvalue_binop.
+      cbn.
+      break_match_goal.
+      rewrite !translate_ret, interp_cfg_to_L3_ret.
+      apply eutt_Ret; cbn; auto.
+      break_match_hyp; try inv_sum.
+      break_match_hyp; try inv_sum.
+      break_match_goal.
+      rewrite translate_raiseUB; apply UB_is_pure.
+      break_match_goal.
+      rewrite translate_raise; apply failure_is_pure.
+      rewrite !translate_ret, interp_cfg_to_L3_ret.
+      apply eutt_Ret; cbn; auto.
+
+  - rewrite translate_bind, interp_cfg_to_L3_bind.
+    eapply has_post_bind_strong.
+    apply (IHe1 (Some t) g l m).
+    intros (? & ? & ? & ?) (-> & -> & ->).
+    rewrite translate_bind, interp_cfg_to_L3_bind.
+    eapply has_post_bind_strong.
+    apply (IHe2 (Some t) g l m).
+    intros (? & ? & ? & ?) (-> & -> & ->).
+    unfold uvalue_to_dvalue_binop.
+    cbn.
+    break_match_goal.
+    rewrite !translate_ret, interp_cfg_to_L3_ret.
+    apply eutt_Ret; cbn; auto.
+    break_match_hyp; try inv_sum.
+    break_match_hyp; try inv_sum.
+    break_match_goal.
+    apply UB_is_pure.
+    break_match_goal.
+    apply failure_is_pure.
+    rewrite !translate_ret, interp_cfg_to_L3_ret.
+    apply eutt_Ret; cbn; auto.
+
+  - rewrite translate_bind, interp_cfg_to_L3_bind.
+    eapply has_post_bind_strong.
+    apply (IHe1 (Some t) g l m).
+    intros (? & ? & ? & ?) (-> & -> & ->).
+    rewrite translate_bind, interp_cfg_to_L3_bind.
+    eapply has_post_bind_strong.
+    apply (IHe2 (Some t) g l m).
+    intros (? & ? & ? & ?) (-> & -> & ->).
+    break_match_goal.
+    + rewrite translate_bind, interp_cfg_to_L3_bind.
+      apply has_post_bind_strong with (↑ (pure_P g l m)).
+      * unfold concretize_or_pick.
+        break_match_goal.
+        cbn.
+        {
+          unfold lift_err.
+          break_match_goal.
+          apply failure_is_pure.
+          rewrite translate_ret, interp_cfg_to_L3_ret.
+          apply eutt_Ret; cbn; auto.
+        }
+       apply pick_is_pure.
+
+      * intros (? & ? & ? & ?) (-> & -> & ->).
+        unfold uvalue_to_dvalue_binop2.
+        cbn; break_match_goal.
+        rewrite translate_ret, interp_cfg_to_L3_ret.
+        apply eutt_Ret; cbn; auto.
+        break_match_hyp; inv_sum.
+        break_match_goal.
+        rewrite translate_raiseUB; apply UB_is_pure.
+        break_match_goal.
+        rewrite translate_raise; apply failure_is_pure.
+        rewrite !translate_ret, interp_cfg_to_L3_ret.
+        apply eutt_Ret; cbn; auto.
+
+    + unfold uvalue_to_dvalue_binop.
+      cbn.
+      break_match_goal.
+      rewrite !translate_ret, interp_cfg_to_L3_ret.
+      apply eutt_Ret; cbn; auto.
+      break_match_hyp; try inv_sum.
+      break_match_hyp; try inv_sum.
+      break_match_goal.
+      rewrite translate_raiseUB; apply UB_is_pure.
+      break_match_goal.
+      rewrite translate_raise; apply failure_is_pure.
+      rewrite !translate_ret, interp_cfg_to_L3_ret.
+      apply eutt_Ret; cbn; auto.
+
+  - rewrite translate_bind, interp_cfg_to_L3_bind.
+    eapply has_post_bind_strong.
+    apply (IHe1 (Some t) g l m).
+    intros (? & ? & ? & ?) (-> & -> & ->).
+    rewrite translate_bind, interp_cfg_to_L3_bind.
+    eapply has_post_bind_strong.
+    apply (IHe2 (Some t) g l m).
+    intros (? & ? & ? & ?) (-> & -> & ->).
+    unfold uvalue_to_dvalue_binop.
+    cbn.
+    break_match_goal.
+    rewrite !translate_ret, interp_cfg_to_L3_ret.
+    apply eutt_Ret; cbn; auto.
+    break_match_hyp; try inv_sum.
+    break_match_hyp; try inv_sum.
+    break_match_goal.
+    apply UB_is_pure.
+    break_match_goal.
+    apply failure_is_pure.
+    rewrite !translate_ret, interp_cfg_to_L3_ret.
+    apply eutt_Ret; cbn; auto.
+
+  - rewrite translate_bind, interp_cfg_to_L3_bind.
+    eapply has_post_bind_strong.
+    apply (IHe (Some t_from) g l m).
+    intros (? & ? & ? & ?) (-> & -> & ->).
+    unfold uvalue_to_dvalue_uop; cbn.
+    break_match_goal.
+    rewrite !translate_ret, interp_cfg_to_L3_ret.
+    apply eutt_Ret; cbn; auto.
+    break_match_hyp; try inv_sum.
+    unfold ITree.map.
+    rewrite !translate_bind, interp_cfg_to_L3_bind.
+    apply has_post_bind_strong with (↑ (pure_P g l m)).
+    + (* What's the right way to reason about eval_conv? *)
+      admit.
+    + intros (? & ? & ? & ?) (-> & -> & ->).
+      rewrite !translate_ret, interp_cfg_to_L3_ret.
+      apply eutt_Ret; cbn; auto.
+
+  - destruct ptrval; cbn.
+    rewrite translate_bind, interp_cfg_to_L3_bind.
+    eapply has_post_bind_strong.
+    apply (IHe (Some d) g l m).
+    intros (? & ? & ? & ?) (-> & -> & ->).
+    rewrite translate_bind, interp_cfg_to_L3_bind.
+    rewrite translate_map_monad.
+    rewrite interp_cfg_to_L3_map_monad.
+    apply has_post_bind_strong with (S := ↑ (pure_P g l m)).
+    + eapply has_post_weaken.
+      apply (map_monad_eutt_state3_ind (fun g' l' m' => pure_P g l m (m',(l',g')))); [| cbn; intuition].
+      * intros * IN (-> & -> & ->).
+        destruct a; simpl in *.
+        apply has_post_weaken with (↑ (pure_P g l m)).
+        apply (H _ IN).
+        intros (? & ? & ? & ?) (-> & -> & ->); auto.
+      * intros (? & ? & ? & ?) (-> & -> & ->); cbn; auto.
+    + intros (? & ? & ? & ?) (-> & -> & ->).
+      break_match_goal.
+      * rewrite translate_bind, interp_cfg_to_L3_bind.
+        unfold concretize_or_pick.
+        apply has_post_bind_strong with (↑ (pure_P g l m)).
+        {
+          break_match_goal.
+          unfold lift_err.
+          break_match_goal.
+          apply failure_is_pure.
+          cbn; rewrite translate_ret, interp_cfg_to_L3_ret; apply eutt_Ret; cbn; auto.
+          apply pick_is_pure.
+        }
+        intros (? & ? & ? & ?) (-> & -> & ->).
+        rewrite translate_bind, interp_cfg_to_L3_bind.
+        rewrite translate_map_monad.
+        rewrite interp_cfg_to_L3_map_monad.
+        apply has_post_bind_strong with (S := ↑ (pure_P g l m)).
+        { eapply has_post_weaken.
+          apply (map_monad_eutt_state3_ind (fun g' l' m' => pure_P g l m (m',(l',g')))); [| cbn; intuition].
+          * intros * IN (-> & -> & ->).
+            break_match_goal.
+            unfold lift_err.
+            break_match_goal.
+            apply failure_is_pure.
+            cbn; rewrite translate_ret, interp_cfg_to_L3_ret; apply eutt_Ret; cbn; auto.
+            apply pick_is_pure.
+          * intros (? & ? & ? & ?) (-> & -> & ->); cbn; auto.
+        }
+        intros (? & ? & ? & ?) (-> & -> & ->); cbn; auto.
+        unfold ITree.map. rewrite translate_bind, interp_cfg_to_L3_bind.
+        rewrite translate_trigger, exp_E_to_instr_E_Memory, subevent_subevent.
+        (* GEP... *)
+        unfold interp_cfg_to_L3.
+        rewrite interp_intrinsics_trigger.
+        cbn.
+        unfold Intrinsics.F_trigger; cbn.
+        rewrite subevent_subevent.
+        rewrite interp_global_trigger; cbn.
+        rewrite subevent_subevent.
+        rewrite interp_local_bind, interp_local_trigger; cbn.
+        rewrite subevent_subevent, bind_bind.
+        rewrite interp_memory_bind, interp_memory_trigger; cbn.
+        rewrite !bind_bind.
+        destruct d0; cbn; try (unfold raise; rewrite bind_bind; apply has_post_bind; intros []).
+        break_match_goal; cbn; try (unfold raise; rewrite bind_bind; apply has_post_bind; intros []).
+        rewrite !bind_ret_l.
+        rewrite interp_local_ret, interp_memory_ret, bind_ret_l.
+        rewrite translate_ret, interp_intrinsics_ret, interp_global_ret, interp_local_ret, interp_memory_ret. 
+        apply eutt_Ret; cbn; auto.
+
+      * unfold ITree.map; destruct p; cbn.
+        rewrite translate_bind, interp_cfg_to_L3_bind.
+        rewrite translate_trigger, exp_E_to_instr_E_Memory, subevent_subevent.
+        (* GEP... *)
+        unfold interp_cfg_to_L3.
+        rewrite interp_intrinsics_trigger.
+        cbn.
+        unfold Intrinsics.F_trigger; cbn.
+        rewrite subevent_subevent.
+        rewrite interp_global_trigger; cbn.
+        rewrite subevent_subevent.
+        rewrite interp_local_bind, interp_local_trigger; cbn.
+        rewrite subevent_subevent, bind_bind.
+        rewrite interp_memory_bind, interp_memory_trigger; cbn.
+        rewrite !bind_bind.
+        destruct d0; cbn; try (unfold raise; rewrite bind_bind; apply has_post_bind; intros []).
+        break_match_goal; cbn; try (unfold raise; rewrite bind_bind; apply has_post_bind; intros []).
+        rewrite !bind_ret_l.
+        rewrite interp_local_ret, interp_memory_ret, bind_ret_l.
+        rewrite translate_ret, interp_intrinsics_ret, interp_global_ret, interp_local_ret, interp_memory_ret. 
+        apply eutt_Ret; cbn; auto.
+
+  - apply failure_is_pure.
+
+  - apply failure_is_pure.
+
+  - apply failure_is_pure.
+
+  - destruct vec; cbn.
+    rewrite translate_bind, interp_cfg_to_L3_bind.
+    eapply has_post_bind_strong.
+    apply (IHe (Some d) g l m).
+    intros (? & ? & ? & ?) (-> & -> & ->).
+    clear IHe.
+    induction idxs as [| n idxs IH].
+    + cbn.
+      rewrite !translate_ret, interp_cfg_to_L3_ret.
+      apply eutt_Ret; cbn; auto.
+    + cbn.
+      break_match_goal.
+      apply UB_is_pure.
+      break_match_goal.
+      apply failure_is_pure.
+      rewrite !translate_ret, interp_cfg_to_L3_ret.
+      apply eutt_Ret; cbn; auto.
+ 
+  - apply failure_is_pure.
+
+  - destruct cnd,v1,v2; cbn.
+    rewrite translate_bind, interp_cfg_to_L3_bind.
+    eapply has_post_bind_strong; [apply IHe | ].
+    intros (? & ? & ? & ?) (-> & -> & ->).
+    rewrite translate_bind, interp_cfg_to_L3_bind.
+    eapply has_post_bind_strong; [apply IHe0 |]. 
+    intros (? & ? & ? & ?) (-> & -> & ->).
+    rewrite translate_bind, interp_cfg_to_L3_bind.
+    eapply has_post_bind_strong; [apply IHe1 |]. 
+    intros (? & ? & ? & ?) (-> & -> & ->).
+    break_match_goal.
+    rewrite !translate_ret, interp_cfg_to_L3_ret.
+    apply eutt_Ret; cbn; auto.
+    unfold lift_undef_or_err.
+    break_match_goal.
+    break_match_goal.
+    apply UB_is_pure.
+    break_match_goal.
+    apply failure_is_pure.
+    rewrite !translate_ret, interp_cfg_to_L3_ret.
+    apply eutt_Ret; cbn; auto.
+    
+  - destruct v; cbn.
+    rewrite translate_bind, interp_cfg_to_L3_bind.
+    eapply has_post_bind_strong.
+    apply (IHe (Some d) g l m).
+    intros (? & ? & ? & ?) (-> & -> & ->).
+    clear IHe.
+    rewrite translate_bind, interp_cfg_to_L3_bind.
+    apply has_post_bind_strong with (↑ (pure_P g l m)).
+    { unfold pick_your_poison;
+      break_match_goal; cbn;
+      match goal with
+        |- context [Ret _] => rewrite !translate_ret, interp_cfg_to_L3_ret; apply eutt_Ret; cbn; auto
+      | |- context [pick] => apply pick_is_pure
+      | |- context [concretize_or_pick] => apply concretize_or_pick_is_pure
+      end.
+    }
+    intros (? & ? & ? & ?) (-> & -> & ->).
+    rewrite !translate_ret, interp_cfg_to_L3_ret.
+    apply eutt_Ret; cbn; auto.
+     
 Admitted.
 
